hol/symb_exec/p4_symb_execLib.sig
@@ -8,27 +8,28 @@ val p4_symb_exec:
    hol_type ->
      (thm * term) ->
        (term * term * term) ->
-         string list -> 
-	   term ->
-	     term list ->
-	       term list -> thm list -> thm -> (thm -> bool) option -> int -> symb_execLib.path_tree * (int * thm * thm) list
+         string list ->
+           thm list ->
+	     term ->
+	       term list ->
+		 term list -> thm list -> thm -> (thm -> bool) option -> int -> symb_execLib.path_tree * (int * thm * thm) list
 
 val p4_symb_exec_prove_contract:
    bool ->
    hol_type ->
-     term -> (term * term * term) -> string list -> term -> term list -> term list -> thm list -> thm -> (thm -> bool) option -> int -> term -> thm
+     term -> (term * term * term) -> string list -> thm list -> term -> term list -> term list -> thm list -> thm -> (thm -> bool) option -> int -> term -> thm
 
 val p4_symb_exec_prove_contract_conc:
    bool ->
    hol_type ->
-     term -> (term * term * term) -> string list ->
+     term -> (term * term * term) -> string list -> thm list ->
        term -> term list -> term list -> thm list -> thm -> (thm -> bool) option -> int -> term -> thm
 
 val p4_debug_symb_exec:
    hol_type ->
      term ->
        (term * term * term) -> 
-         string list -> 
+         string list -> thm list ->
 	   term ->
 	     term list ->
 	       term list ->
@@ -42,7 +43,7 @@ val p4_debug_symb_exec_frame_lists:
    hol_type ->
      term ->
        (term * term * term) ->
-         string list -> 
+         string list -> thm list ->
 	   term ->
 	     term list ->
 	       term list -> thm list -> thm -> int -> symb_execLib.path_tree * term list
