hol/symb_exec/p4_symb_exec_test3Script.sml
@@ -152,6 +152,7 @@ val arch_ty = p4_v1modelLib.v1model_arch_ty
 val ctx = symb_exec3_actx
 val (fty_map, b_fty_map, pblock_action_names_map) = (symb_exec3_ftymap, symb_exec3_blftymap, symb_exec3_pblock_action_names_map)
 val const_actions_tables = []
+val path_cond_defs = []
 val init_astate = symb_exec3_astate_symb
 val stop_consts_rewr = []
 val stop_consts_never = []
@@ -175,6 +176,6 @@ val [(path_cond_res, step_thm), (path_cond2_res, step_thm2)] =
 
 (* Finishes at 45 steps (one step of which is a symbolic branch)
  * (higher numbers as arguments will work, but do no extra computations) *)
-val contract_thm = p4_symb_exec_prove_contract_conc debug_flag arch_ty ctx (fty_map, b_fty_map, pblock_action_names_map) const_actions_tables init_astate stop_consts_rewr stop_consts_never [] path_cond p4_is_finished_alt_opt n_max postcond;
+val contract_thm = p4_symb_exec_prove_contract_conc debug_flag arch_ty ctx (fty_map, b_fty_map, pblock_action_names_map) const_actions_tables path_cond_defs init_astate stop_consts_rewr stop_consts_never [] path_cond p4_is_finished_alt_opt n_max postcond;
 
 val _ = export_theory ();
